src/computational_monads/simulation_semantics/is_tracking.lean
@@ -14,6 +14,9 @@ This is represented by giving functions `query_f` and `state_f` that correspond 
 and a statement `apply_dist_equiv_state_f_map_query_f` that shows that the oracle function
 actually splits into the two components given.
 
+Note that we require that `query_f` be deterministic for simplicity.
+For current use cases this is generally sufficient.
+
 For example in `loggingₛₒ` the internal state doesn't change the main output, it just records it.
 This allows for many lemmas to be automatically shared between these sorts of oracles.
 `sim_oracle.is_stateless` extends this further to oracles with no internal state at all.
@@ -24,11 +27,11 @@ This is convenient in defining e.g. `loggingₛₒ` and `idₛₒ`
 -/
 
 open_locale big_operators ennreal
-open oracle_comp oracle_spec
-
-namespace sim_oracle
+open oracle_comp oracle_spec prod
 
 variables {α β γ : Type} {spec spec' spec'' : oracle_spec} {S S' : Type}
+
+namespace sim_oracle
 
 /-- Typeclass for oracles in which the query responses are independent of the current oracle state.
 We define this in terms of the existence of two functions `query_f` and `state_f`
@@ -40,8 +43,7 @@ class is_tracking (so : sim_oracle spec spec' S) :=
 (apply_dist_equiv_state_f_map_query_f : ∀ (i : spec.ι) (t : spec.domain i) (s : S),
   so i (t, s) ≃ₚ (λ u, (u, state_f s i t u)) <$> query_f i t)
 
-variables (so : sim_oracle spec spec' S) (oa : oracle_comp spec α) (i : spec.ι)
-  (t t' : spec.domain i) (s s' : S) (u u' : spec.range i)
+variables (so : sim_oracle spec spec' S) (so' : sim_oracle spec spec'' S')
 
 /-- Alias to be able to refer to the query function from the `sim_oracle` namespace. -/
 @[inline, reducible] def answer_query [hso : so.is_tracking] (i : spec.ι) (t : spec.domain i) :
@@ -53,72 +55,57 @@ variables (so : sim_oracle spec spec' S) (oa : oracle_comp spec α) (i : spec.ι
 
 namespace is_tracking
 
-variable [hso : so.is_tracking]
+section apply
+
+variables [hso : so.is_tracking] {i : spec.ι} (t : spec.domain i) (s : S)
 include hso
 
 @[pairwise_dist_equiv] lemma apply_dist_equiv : so i (t, s) ≃ₚ
   (λ u, (u, so.update_state s i t u)) <$> so.answer_query i t :=
 is_tracking.apply_dist_equiv_state_f_map_query_f i t s
 
-section support
-
-lemma support_apply' : (so i (t, s)).support =
-  ((λ u, (u, so.update_state s i t u)) <$> so.answer_query i t).support :=
-by simp_rw [← support_eval_dist, (hso.apply_dist_equiv_state_f_map_query_f _ _ _).eval_dist_eq]
-
 @[simp] lemma support_apply : (so i (t, s)).support =
   (λ u, (u, so.update_state s i t u)) '' (so.answer_query i t).support :=
-by rw [support_apply', support_map]
-
-end support
-
-section fin_support
-
-lemma fin_support_apply' [decidable_eq S] : (so i (t, s)).fin_support =
-  ((λ u, (u, so.update_state s i t u)) <$> so.answer_query i t).fin_support :=
-by rw [fin_support_eq_fin_support_iff_support_eq_support, support_apply']
+(apply_dist_equiv so t s).support_eq.trans (by rw [support_map])
 
 @[simp] lemma fin_support_apply [decidable_eq S] : (so i (t, s)).fin_support =
   (so.answer_query i t).fin_support.image (λ u, (u, so.update_state s i t u)) :=
-by rw [fin_support_apply', fin_support_map]
-
-end fin_support
-
-section eval_dist
-
-lemma eval_dist_apply' : ⁅so i (t, s)⁆ =
-  ⁅(λ u, (u, so.update_state s i t u)) <$> so.answer_query i t⁆ :=
-apply_dist_equiv_state_f_map_query_f i t s
+(apply_dist_equiv so t s).fin_support_eq.trans (by rw [fin_support_map])
 
 @[simp] lemma eval_dist_apply : ⁅so i (t, s)⁆ =
   ⁅so.answer_query i t⁆.map (λ u, (u, so.update_state s i t u)) :=
-by rw [eval_dist_apply', eval_dist_map]
+(apply_dist_equiv so t s).eval_dist_eq.trans (by rw [eval_dist_map])
 
-end eval_dist
-
-section prob_event
-
-lemma prob_event_apply' (e : set (spec.range i × S)) : ⁅e | so i (t, s)⁆ =
-  ⁅e | (λ u, (u, so.update_state s i t u)) <$> so.answer_query i t⁆ :=
-prob_event_eq_of_eval_dist_eq (eval_dist_apply' so i t s) e
+@[simp] lemma prob_output_apply (z : spec.range i × S) : ⁅= z | so i (t, s)⁆ =
+  ⁅λ u, (u, so.update_state s i t u) = z | so.answer_query i t⁆ :=
+((apply_dist_equiv so t s).prob_output_eq z).trans
+  (by simpa only [← prob_event_singleton_eq_prob_output, prob_event_map])
 
 @[simp] lemma prob_event_apply (e : set (spec.range i × S)) : ⁅e | so i (t, s)⁆ =
   ⁅(λ u, (u, so.update_state s i t u)) ⁻¹' e | so.answer_query i t⁆ :=
-by rw [prob_event_apply', prob_event_map]
+((apply_dist_equiv so t s).prob_event_eq e).trans (by rw [prob_event_map])
 
-end prob_event
+end apply
 
-section simulate'
+section simulate_idem
 
-/-- If the oracle can take on any value then the first element of the support is unchanged -/
-lemma support_simulate'_eq_support (h : ∀ i t, (so.answer_query i t).support = set.univ) :
+variables [hso : so.is_tracking] (oa : oracle_comp spec α) (s : S)
+include hso
+
+/-- If `so.answer_query` can take on any value then the support of simulation with `so` can give
+any output that the original computation did (excluding the state). -/
+lemma support_simulate'_eq_support
+  (h : ∀ i (t : spec.domain i), (so.answer_query i t).support = set.univ) :
   (simulate' so oa s).support = oa.support :=
-sorry
--- support_simulate'_eq_support _ oa s (λ i t s, set.ext (λ x, by simp_rw [is_tracking.support_apply,
---   set.image_image, h, set.image_univ, set.range_id', set.top_eq_univ]))
+begin
+  refine support_simulate'_eq_support oa s (λ i t s, _),
+  rw [is_tracking.support_apply, ← set.image_comp, h],
+  exact set.image_univ_of_surjective (λ u, ⟨u, refl u⟩),
+end
 
+/-- Version of `support_simulate'_eq_support` for `fin_support`. -/
 lemma fin_support_simulate'_eq_fin_support
-  (h : ∀ i t, (so.answer_query i t).fin_support = finset.univ) :
+  (h : ∀ i (t : spec.domain i), (so.answer_query i t).fin_support = finset.univ) :
   (simulate' so oa s).fin_support = oa.fin_support :=
 begin
   rw [fin_support_eq_fin_support_iff_support_eq_support],
@@ -126,23 +113,63 @@ begin
   rw [← coe_fin_support_eq_support, h i t, finset.coe_univ]
 end
 
-lemma simulate'_dist_equiv_self (h : ∀ i t, so.answer_query i t ≃ₚ query i t) :
+/-- If `so.answer_query` looks like just calling `query` then the distribution of the non-state
+portion of simulation by `so` is distributionally equivalent to the original computation. -/
+lemma simulate'_dist_equiv_self
+  (h : ∀ i (t : spec.domain i), so.answer_query i t ≃ₚ query i t) :
   simulate' so oa s ≃ₚ oa :=
 begin
-  sorry,
-  -- refine simulate'_dist_equiv_s
+  refine simulate'_dist_equiv_self oa s (λ i t s, _),
+  rw_dist_equiv [is_tracking.apply_dist_equiv, map_comp_dist_equiv, bind_return_id_dist_equiv],
+  exact h i t,
 end
 
-
+/-- If the distribution of `so.answer_query` is uniform, then the distribution of the first result
+of simulation by `so` looks like that of the original computation. -/
 lemma eval_dist_simulate'_eq_eval_dist
   (h : ∀ i t, ⁅so.answer_query i t⁆ = pmf.uniform_of_fintype (spec.range i)) :
   ⁅simulate' so oa s⁆ = ⁅oa⁆ :=
+is_tracking.simulate'_dist_equiv_self so oa s
+  (λ i t, (h i t).trans (eval_dist_query i t).symm)
+
+/-- If all outputs of `so.answer_query` have the same probability, then the first output of
+simulation with `so` has the same probability as in the original computation. -/
+lemma prob_output_simulate'_eq_prob_output
+  (h : ∀ i t u, ⁅= u | so.answer_query i t⁆ = (fintype.card (spec.range i))⁻¹)
+  (x : α) : ⁅= x | simulate' so oa s⁆ = ⁅= x | oa⁆ :=
 begin
-  sorry,
-  -- refine eval_dist_simulate'_eq_eval_dist so oa s (λ i t s, _),
+  refine (simulate'_dist_equiv_self so oa s (λ i t, _)).prob_output_eq x,
+  simp only [dist_equiv.ext_iff, h, prob_output_query_eq_inv, forall_const],
 end
 
-end simulate'
+/-- If all outputs of `so.answer_query` have the same probability, then the first output of
+simulation with `so` has the same probability as in the original computation. -/
+lemma prob_event_simulate'_eq_prob_event
+  (h : ∀ i t u, ⁅= u | so.answer_query i t⁆ = (fintype.card (spec.range i))⁻¹)
+  (e : set α) : ⁅e | simulate' so oa s⁆ = ⁅e | oa⁆ :=
+begin
+  refine (simulate'_dist_equiv_self so oa s (λ i t, _)).prob_event_eq e,
+  simp only [dist_equiv.ext_iff, h, prob_output_query_eq_inv, forall_const],
+end
+
+end simulate_idem
+
+section simulate_eq_simulate
+
+variables [hso : so.is_tracking] [hso' : so'.is_tracking]
+  (oa : oracle_comp spec α) (s : S) (s' : S')
+include hso hso'
+
+lemma simulate'_dist_equiv_simulate'
+  (h : ∀ i t, so.answer_query i t ≃ₚ so'.answer_query i t) :
+  simulate' so oa s ≃ₚ simulate' so' oa s' :=
+begin
+  refine simulate'_dist_equiv_simulate' oa s s' (λ i t s s', _),
+  simp_rw_dist_equiv [is_tracking.apply_dist_equiv, map_comp_dist_equiv],
+  pairwise_dist_equiv [h i t]
+end
+
+end simulate_eq_simulate
 
 end is_tracking
 
@@ -154,169 +181,177 @@ For example a logging oracle that just tracks the input and output of queries.
 `o` is the way the oracle responds to queries, which doesn't have access to the state.
 `update_state` takes a query and internal state and returns the new internal state.
 Note that `update_state` is not a probabalistic function, and has no oracle access -/
-def tracking_oracle {spec spec' : oracle_spec} {S : Type}
-  (o : Π (i : spec.ι), spec.domain i → oracle_comp spec' (spec.range i))
-  (update_state : Π (s : S) (i : spec.ι), spec.domain i → spec.range i → S)
+def tracking_oracle (query_f : Π (i : spec.ι), spec.domain i → oracle_comp spec' (spec.range i))
+  (state_f : Π (s : S) (i : spec.ι), spec.domain i → spec.range i → S)
   (default_state : S) : sim_oracle spec spec' S :=
 { default_state := default_state,
-  o := λ i ⟨t, s⟩, (λ u, (u, update_state s i t u)) <$> (o i t) }
+  o := λ i ⟨t, s⟩, (λ u, (u, state_f s i t u)) <$> (query_f i t) }
 
-notation `⟪` o `|` update_state `,` default_state `⟫` :=
-  tracking_oracle o update_state default_state
+notation `⟪` query_f `|` state_f `,` default_state `⟫` :=
+  tracking_oracle query_f state_f default_state
 
-namespace tracking_oracle
+instance tacking_oracle.is_tracking
+  (query_f : Π (i : spec.ι), spec.domain i → oracle_comp spec' (spec.range i))
+  (state_f : Π (s : S) (i : spec.ι), spec.domain i → spec.range i → S)
+  (default_state : S) : ⟪query_f | state_f, default_state⟫.is_tracking :=
+{ query_f := query_f,
+  state_f := state_f,
+  apply_dist_equiv_state_f_map_query_f := λ i t s, dist_equiv.rfl }
 
-open_locale big_operators ennreal
-open oracle_comp oracle_spec
 
-variables {α β γ : Type} {spec spec' spec'' : oracle_spec}
-variables {S S' : Type} (o : Π (i : spec.ι), spec.domain i → oracle_comp spec' (spec.range i))
-  (o' : Π (i : spec.ι), spec.domain i → oracle_comp spec'' (spec.range i))
-  (update_state : Π (s : S) (i : spec.ι), spec.domain i → spec.range i → S)
-  (update_state' : Π (s : S') (i : spec.ι), spec.domain i → spec.range i → S')
-  (default_state : S) (default_state' : S') (a : α) (i : spec.ι) (t : spec.domain i)
-  (oa : oracle_comp spec α) (ob : α → oracle_comp spec β) (s : S) (s' : S')
-  (x : spec.domain i × S) (y : spec.range i × S)
+-- namespace tracking_oracle
 
-@[simp] lemma apply_eq : ⟪o | update_state, default_state⟫ i x =
-  (λ u, (u, update_state x.2 i x.1 u)) <$> (o i x.1) := by {cases x, refl}
+-- open_locale big_operators ennreal
+-- open oracle_comp oracle_spec
 
-section support
+-- variables {α β γ : Type} {spec spec' spec'' : oracle_spec}
+-- variables {S S' : Type} (o : Π (i : spec.ι), spec.domain i → oracle_comp spec' (spec.range i))
+--   (o' : Π (i : spec.ι), spec.domain i → oracle_comp spec'' (spec.range i))
+--   (update_state : Π (s : S) (i : spec.ι), spec.domain i → spec.range i → S)
+--   (update_state' : Π (s : S') (i : spec.ι), spec.domain i → spec.range i → S')
+--   (default_state : S) (default_state' : S') (a : α) (i : spec.ι) (t : spec.domain i)
+--   (oa : oracle_comp spec α) (ob : α → oracle_comp spec β) (s : S) (s' : S')
+--   (x : spec.domain i × S) (y : spec.range i × S)
 
-@[simp] lemma support_apply : (⟪o | update_state, default_state⟫ i x).support =
-  (λ u, (u, update_state x.2 i x.1 u)) '' (o i x.1).support :=
-set.ext (λ y, by rw [apply_eq, support_map])
+-- @[simp] lemma apply_eq : ⟪o | update_state, default_state⟫ i x =
+--   (λ u, (u, update_state x.2 i x.1 u)) <$> (o i x.1) := by {cases x, refl}
 
-lemma fin_support_apply [decidable_eq S] :
-  (⟪o | update_state, default_state⟫ i x).fin_support =
-    (o i x.1).fin_support.image (λ u, (u, update_state x.2 i x.1 u)) :=
-by simp only [fin_support_eq_iff_support_eq_coe, apply_eq, support_map,
-  finset.coe_image, coe_fin_support_eq_support]
+-- section support
 
-lemma mem_support_apply_iff {y : spec.range i × S} :
-  y ∈ (⟪o | update_state, default_state⟫ i x).support ↔
-    y.1 ∈ (o i x.1).support ∧ update_state x.2 i x.1 y.1 = y.2 :=
-by simp only [support_apply, prod.eq_iff_fst_eq_snd_eq, set.mem_image,
-  and_comm (_ = y.fst), exists_eq_right_right]
+-- @[simp] lemma support_apply : (⟪o | update_state, default_state⟫ i x).support =
+--   (λ u, (u, update_state x.2 i x.1 u)) '' (o i x.1).support :=
+-- set.ext (λ y, by rw [apply_eq, support_map])
 
-/-- If the oracle can take on any value then the first element of the support is unchanged -/
-lemma support_simulate'_eq_support (h : ∀ i t, (o i t).support = ⊤) :
-  (simulate' ⟪o | update_state, default_state⟫ oa s).support = oa.support :=
-sorry
--- support_simulate'_eq_support _ oa s (λ i t s, set.ext (λ x, by simp only
---   [h, set.top_eq_univ, set.mem_univ, true_and, apply_eq, support_map, set.mem_image,
---     prod.exists, prod.mk.inj_iff, exists_eq_left, exists_eq_left', exists_apply_eq_apply]))
+-- lemma fin_support_apply [decidable_eq S] :
+--   (⟪o | update_state, default_state⟫ i x).fin_support =
+--     (o i x.1).fin_support.image (λ u, (u, update_state x.2 i x.1 u)) :=
+-- by simp only [fin_support_eq_iff_support_eq_coe, apply_eq, support_map,
+--   finset.coe_image, coe_fin_support_eq_support]
 
-/-- Particular case of `support_simulate'_eq_support` for `query`.
-In particular a tracking oracle that *only* does tracking doesn't affect the main output. -/
-@[simp] lemma support_simulate'_query_eq_support :
-  (simulate' ⟪query | update_state, default_state⟫ oa s).support = oa.support :=
-support_simulate'_eq_support query update_state default_state oa s (λ _ _, rfl)
+-- lemma mem_support_apply_iff {y : spec.range i × S} :
+--   y ∈ (⟪o | update_state, default_state⟫ i x).support ↔
+--     y.1 ∈ (o i x.1).support ∧ update_state x.2 i x.1 y.1 = y.2 :=
+-- by simp only [support_apply, prod.eq_iff_fst_eq_snd_eq, set.mem_image,
+--   and_comm (_ = y.fst), exists_eq_right_right]
 
-lemma support_simulate'_eq_support_simulate' (h : ∀ i t, (o i t).support = (o' i t).support) :
-  (simulate' ⟪o | update_state, default_state⟫ oa s).support =
-    (simulate' ⟪o' | update_state', default_state'⟫ oa s').support :=
-support_simulate'_eq_support_simulate' oa s s' (λ i t s s', set.ext (λ x,
-  by simp only [mem_support_apply_iff, h, simulate'_query, support_map, support_apply,
-    set.mem_image, set.mem_set_of_eq, prod.exists, exists_and_distrib_right, exists_eq_right,
-    exists_eq_right', exists_eq_right_right, prod.eq_iff_fst_eq_snd_eq, and_comm (_ = x)]))
+-- /-- If the oracle can take on any value then the first element of the support is unchanged -/
+-- lemma support_simulate'_eq_support (h : ∀ i t, (o i t).support = ⊤) :
+--   (simulate' ⟪o | update_state, default_state⟫ oa s).support = oa.support :=
+-- sorry
+-- -- support_simulate'_eq_support _ oa s (λ i t s, set.ext (λ x, by simp only
+-- --   [h, set.top_eq_univ, set.mem_univ, true_and, apply_eq, support_map, set.mem_image,
+-- --     prod.exists, prod.mk.inj_iff, exists_eq_left, exists_eq_left', exists_apply_eq_apply]))
 
-/-- The support of `simulate'` is independt of the tracking functions -/
-lemma support_simulate'_eq_support_simulate'_of_oracle_eq :
-  (simulate' ⟪o | update_state, default_state⟫ oa s).support =
-    (simulate' ⟪o | update_state', default_state'⟫ oa s').support :=
-support_simulate'_eq_support_simulate' o o _ _ _ _ oa s s' (λ _ _, rfl)
+-- /-- Particular case of `support_simulate'_eq_support` for `query`.
+-- In particular a tracking oracle that *only* does tracking doesn't affect the main output. -/
+-- @[simp] lemma support_simulate'_query_eq_support :
+--   (simulate' ⟪query | update_state, default_state⟫ oa s).support = oa.support :=
+-- support_simulate'_eq_support query update_state default_state oa s (λ _ _, rfl)
 
-section subsingleton
+-- lemma support_simulate'_eq_support_simulate' (h : ∀ i t, (o i t).support = (o' i t).support) :
+--   (simulate' ⟪o | update_state, default_state⟫ oa s).support =
+--     (simulate' ⟪o' | update_state', default_state'⟫ oa s').support :=
+-- support_simulate'_eq_support_simulate' oa s s' (λ i t s s', set.ext (λ x,
+--   by simp only [mem_support_apply_iff, h, simulate'_query, support_map, support_apply,
+--     set.mem_image, set.mem_set_of_eq, prod.exists, exists_and_distrib_right, exists_eq_right,
+--     exists_eq_right', exists_eq_right_right, prod.eq_iff_fst_eq_snd_eq, and_comm (_ = x)]))
 
-variables [subsingleton S]
+-- /-- The support of `simulate'` is independt of the tracking functions -/
+-- lemma support_simulate'_eq_support_simulate'_of_oracle_eq :
+--   (simulate' ⟪o | update_state, default_state⟫ oa s).support =
+--     (simulate' ⟪o | update_state', default_state'⟫ oa s').support :=
+-- support_simulate'_eq_support_simulate' o o _ _ _ _ oa s s' (λ _ _, rfl)
 
-@[simp] lemma support_apply_of_subsingleton :
-  (⟪o | update_state, default_state⟫ i x).support = prod.fst ⁻¹' (o i x.1).support :=
-set.ext (λ y, by erw [apply_eq, map_eq_bind_return_comp,
-  support_bind_prod_mk_of_snd_subsingleton, set.image_id])
+-- section subsingleton
 
-lemma support_simulate_eq_preimage_support_of_subsingleton (h : ∀ i t, (o i t).support = ⊤) :
-  (simulate ⟪o | update_state, default_state⟫ oa s).support = prod.fst ⁻¹' oa.support :=
-by rw [set.preimage, support_simulate_eq_support_simulate'_of_subsingleton,
-  support_simulate'_eq_support o _ _ oa s h]
+-- variables [subsingleton S]
 
-@[simp] lemma support_simulate_query_eq_support_of_subsingleton :
-  (simulate ⟪query | update_state, default_state⟫ oa s).support = prod.fst ⁻¹' oa.support :=
-support_simulate_eq_preimage_support_of_subsingleton query _ _ oa s (λ _ _, rfl)
+-- @[simp] lemma support_apply_of_subsingleton :
+--   (⟪o | update_state, default_state⟫ i x).support = fst ⁻¹' (o i x.1).support :=
+-- set.ext (λ y, by erw [apply_eq, map_eq_bind_return_comp,
+--   support_bind_prod_mk_of_snd_subsingleton, set.image_id])
 
-end subsingleton
+-- lemma support_simulate_eq_preimage_support_of_subsingleton (h : ∀ i t, (o i t).support = ⊤) :
+--   (simulate ⟪o | update_state, default_state⟫ oa s).support = fst ⁻¹' oa.support :=
+-- by rw [set.preimage, support_simulate_eq_support_simulate'_of_subsingleton,
+--   support_simulate'_eq_support o _ _ oa s h]
 
-end support
+-- @[simp] lemma support_simulate_query_eq_support_of_subsingleton :
+--   (simulate ⟪query | update_state, default_state⟫ oa s).support = fst ⁻¹' oa.support :=
+-- support_simulate_eq_preimage_support_of_subsingleton query _ _ oa s (λ _ _, rfl)
 
-section eval_dist
+-- end subsingleton
 
-@[simp] lemma eval_dist_apply :
-  ⁅⟪o | update_state, default_state⟫ i (t, s)⁆ = ⁅o i t⁆.map (λ u, (u, update_state s i t u)) :=
-by rw [apply_eq, eval_dist_map]
+-- end support
 
-/-- If the oracle has uniform distribution, then the distribution under `simulate'` is unchanged -/
-lemma eval_dist_simulate'_eq_eval_dist
-  (h : ∀ i t, ⁅o i t⁆ = pmf.uniform_of_fintype (spec.range i)) :
-  ⁅simulate' ⟪o | update_state, default_state⟫ oa s⁆ = ⁅oa⁆ :=
-sorry
--- eval_dist_simulate'_eq_eval_dist _ oa s (λ i t s, trans
---   (by simpa [eval_dist_apply, pmf.map_comp] using pmf.map_id ⁅o i t⁆) (h i t))
+-- section eval_dist
 
-/-- Specific case of `eval_dist_simulate'_eq_eval_dist` for query.
-In particular if a tracking oracle *only* does tracking gives the same main output distribution. -/
-@[simp] lemma eval_dist_simulate'_query_eq_eval_dist :
-  ⁅simulate' ⟪query | update_state, default_state⟫ oa s⁆ = ⁅oa⁆ :=
-eval_dist_simulate'_eq_eval_dist query update_state default_state oa s (λ _ _, rfl)
+-- @[simp] lemma eval_dist_apply :
+--   ⁅⟪o | update_state, default_state⟫ i (t, s)⁆ = ⁅o i t⁆.map (λ u, (u, update_state s i t u)) :=
+-- by rw [apply_eq, eval_dist_map]
 
-lemma eval_dist_simulate'_eq_eval_dist_simulate'
-  (h : ∀ i t, o i t ≃ₚ o' i t) : simulate' ⟪o | update_state, default_state⟫ oa s ≃ₚ
-    simulate' ⟪o' | update_state', default_state'⟫ oa s' :=
-sorry
--- -- eval_dist_simulate'_eq_eval_dist_simulate' (λ i t s s',
---   by simp [pmf.map_comp, tracking_oracle.apply_eq, eval_dist_map, (h i t).eval_dist_eq]) _ _ _
+-- /-- If the oracle has uniform distribution, then the distribution under `simulate'` is unchanged -/
+-- lemma eval_dist_simulate'_eq_eval_dist
+--   (h : ∀ i t, ⁅o i t⁆ = pmf.uniform_of_fintype (spec.range i)) :
+--   ⁅simulate' ⟪o | update_state, default_state⟫ oa s⁆ = ⁅oa⁆ :=
+-- sorry
+-- -- eval_dist_simulate'_eq_eval_dist _ oa s (λ i t s, trans
+-- --   (by simpa [eval_dist_apply, pmf.map_comp] using pmf.map_id ⁅o i t⁆) (h i t))
 
-/-- The first output of simulation under different `tracking_oracle` with the same oracle
-is the same regardless of if the tracking functions are different. -/
-lemma eval_dist_simulate'_eq_eval_dist_simulate'_of_oracle_eq :
-  ⁅simulate' ⟪o | update_state, default_state⟫ oa s⁆ =
-    ⁅simulate' ⟪o | update_state', default_state'⟫ oa s'⁆ :=
-eval_dist_simulate'_eq_eval_dist_simulate' o o _ _ _ _ oa s s' (λ _ _, rfl)
+-- /-- Specific case of `eval_dist_simulate'_eq_eval_dist` for query.
+-- In particular if a tracking oracle *only* does tracking gives the same main output distribution. -/
+-- @[simp] lemma eval_dist_simulate'_query_eq_eval_dist :
+--   ⁅simulate' ⟪query | update_state, default_state⟫ oa s⁆ = ⁅oa⁆ :=
+-- eval_dist_simulate'_eq_eval_dist query update_state default_state oa s (λ _ _, rfl)
 
-end eval_dist
+-- lemma eval_dist_simulate'_eq_eval_dist_simulate'
+--   (h : ∀ i t, o i t ≃ₚ o' i t) : simulate' ⟪o | update_state, default_state⟫ oa s ≃ₚ
+--     simulate' ⟪o' | update_state', default_state'⟫ oa s' :=
+-- sorry
+-- -- -- eval_dist_simulate'_eq_eval_dist_simulate' (λ i t s s',
+-- --   by simp [pmf.map_comp, tracking_oracle.apply_eq, eval_dist_map, (h i t).eval_dist_eq]) _ _ _
 
-section prob_event
+-- /-- The first output of simulation under different `tracking_oracle` with the same oracle
+-- is the same regardless of if the tracking functions are different. -/
+-- lemma eval_dist_simulate'_eq_eval_dist_simulate'_of_oracle_eq :
+--   ⁅simulate' ⟪o | update_state, default_state⟫ oa s⁆ =
+--     ⁅simulate' ⟪o | update_state', default_state'⟫ oa s'⁆ :=
+-- eval_dist_simulate'_eq_eval_dist_simulate' o o _ _ _ _ oa s s' (λ _ _, rfl)
 
-variable (e : set α)
+-- end eval_dist
 
-@[simp] lemma prob_event_apply (e : set (spec.range i × S)) :
-  ⁅e | ⟪o | update_state, default_state⟫ i (t, s)⁆ =
-    ⁅λ u, (u, update_state s i t u) ∈ e | o i t⁆ :=
-by simpa only [apply_eq, prob_event_map]
+-- section prob_event
 
-lemma prob_event_simulate'_eq_prob_event
-  (h : ∀ i t, ⁅o i t⁆ = pmf.uniform_of_fintype (spec.range i)) :
-  ⁅e | simulate' ⟪o | update_state, default_state⟫ oa s⁆ = ⁅e | oa⁆ :=
-prob_event_eq_of_eval_dist_eq (eval_dist_simulate'_eq_eval_dist _ _ _ _ _ h) e
+-- variable (e : set α)
 
-/-- Specific case of `eval_dist_simulate'_eq_eval_dist` for query.
-In particular if a tracking oracle *only* does tracking gives the same main output distribution. -/
-lemma prob_event_simulate'_query_eq_prob_event :
-  ⁅e | simulate' ⟪query | update_state, default_state⟫ oa s⁆ = ⁅e | oa⁆ :=
-prob_event_simulate'_eq_prob_event _ _ _ oa s e (λ _ _, rfl)
+-- @[simp] lemma prob_event_apply (e : set (spec.range i × S)) :
+--   ⁅e | ⟪o | update_state, default_state⟫ i (t, s)⁆ =
+--     ⁅λ u, (u, update_state s i t u) ∈ e | o i t⁆ :=
+-- by simpa only [apply_eq, prob_event_map]
 
-lemma prob_event_simulate'_eq_prob_event_simulate'
-  (h : ∀ i t, o i t ≃ₚ o' i t) : ⁅e | simulate' ⟪o | update_state, default_state⟫ oa s⁆ =
-    ⁅e | simulate' ⟪o' | update_state', default_state'⟫ oa s'⁆ :=
-prob_event_eq_of_eval_dist_eq (eval_dist_simulate'_eq_eval_dist_simulate' _ _ _ _ _ _ _ _ _ h) e
+-- lemma prob_event_simulate'_eq_prob_event
+--   (h : ∀ i t, ⁅o i t⁆ = pmf.uniform_of_fintype (spec.range i)) :
+--   ⁅e | simulate' ⟪o | update_state, default_state⟫ oa s⁆ = ⁅e | oa⁆ :=
+-- prob_event_eq_of_eval_dist_eq (eval_dist_simulate'_eq_eval_dist _ _ _ _ _ h) e
 
-/-- The first output of simulation under different `tracking_oracle` with the same oracle
-is the same regardless of if the tracking functions are different. -/
-lemma prob_event_simulate'_eq_eval_dist_simulate'_of_oracle_eq :
-  ⁅e | simulate' ⟪o | update_state, default_state⟫ oa s⁆ =
-    ⁅e | simulate' ⟪o | update_state', default_state'⟫ oa s'⁆ :=
-prob_event_simulate'_eq_prob_event_simulate' o o _ _ _ _ oa s s' e (λ _ _, rfl)
+-- /-- Specific case of `eval_dist_simulate'_eq_eval_dist` for query.
+-- In particular if a tracking oracle *only* does tracking gives the same main output distribution. -/
+-- lemma prob_event_simulate'_query_eq_prob_event :
+--   ⁅e | simulate' ⟪query | update_state, default_state⟫ oa s⁆ = ⁅e | oa⁆ :=
+-- prob_event_simulate'_eq_prob_event _ _ _ oa s e (λ _ _, rfl)
 
-end prob_event
+-- lemma prob_event_simulate'_eq_prob_event_simulate'
+--   (h : ∀ i t, o i t ≃ₚ o' i t) : ⁅e | simulate' ⟪o | update_state, default_state⟫ oa s⁆ =
+--     ⁅e | simulate' ⟪o' | update_state', default_state'⟫ oa s'⁆ :=
+-- prob_event_eq_of_eval_dist_eq (eval_dist_simulate'_eq_eval_dist_simulate' _ _ _ _ _ _ _ _ _ h) e
 
-end tracking_oracle
+-- /-- The first output of simulation under different `tracking_oracle` with the same oracle
+-- is the same regardless of if the tracking functions are different. -/
+-- lemma prob_event_simulate'_eq_eval_dist_simulate'_of_oracle_eq :
+--   ⁅e | simulate' ⟪o | update_state, default_state⟫ oa s⁆ =
+--     ⁅e | simulate' ⟪o | update_state', default_state'⟫ oa s'⁆ :=
+-- prob_event_simulate'_eq_prob_event_simulate' o o _ _ _ _ oa s s' e (λ _ _, rfl)
+
+-- end prob_event
+
+-- end tracking_oracle
